GreedyDeriv/Examples.lean
@@ -3,103 +3,123 @@ import GreedyDeriv.Greedy
 
 open Regex
 
-/-- Helper function to convert strings into regexes (string as a sequence of characters) -/
-def String.toRegex (s : String) : Regex Char :=
-  s.toList |>.map char |>.foldr Regex.mul epsilon
-
-/-- Implicit coercion to convert strings to regexes to make them more readable. -/
+/-- Implicit coercion to convert strings to regexes -/
 instance : Coe String (Regex Char) where
-  coe := String.toRegex
+  coe s := s.toList |>.map char |>.foldr Regex.mul epsilon
 
-/-- Implicit coercion to convert characters to regexes to make them more readable -/
+/-- Implicit coercion to convert characters to regexes -/
 instance : Coe Char (Regex Char) where
   coe := char
 
+/-- Implicit coercion to convert strings to initial locations -/
+instance : Coe String (Loc Char) where
+  coe := ([], String.toList ·)
+
 -- a + ab
 def r : Regex (Char) := plus 'a' "ab"
-#eval r.rmatch "ab".toList
-#eval r.gmatch "ab".toList
+#eval r.matchEnd "ab"
+#eval r.gmatch "ab"
 
 -- (a + ab)*
 def r2 : Regex (Char) := (plus 'a' "ab").star false
-#eval r2.rmatch "aab".toList
-#eval r2.gmatch "aab".toList
+#eval r2.matchEnd "aab"
+#eval r2.gmatch "aab"
 
 -- c + ab
 def r3 : Regex (Char) := plus 'c' (mul 'a' 'b')
-#eval r3.rmatch "ab".toList
-#eval r3.gmatch "ab".toList
+#eval r3.matchEnd "ab"
+#eval r3.gmatch "ab"
 
 -- (a + aa)a
 def r4 : Regex (Char) := (plus 'a' "aa").mul 'a'
-#eval r4.rmatch "aaa".toList
-#eval r4.gmatch "aaa".toList
+#eval r4.matchEnd "aaa"
+#eval r4.gmatch "aaa"
 
 -- a*a
 def r5 : Regex (Char) := (star 'a' false).mul 'a'
-#eval r5.rmatch "aa".toList
-#eval r5.gmatch "aa".toList
+#eval r5.matchEnd "aa"
+#eval r5.gmatch "aa"
 
--- (ε|b)*
+-- (ε + b)*
 def r6 : Regex (Char) := (epsilon.plus 'b').star false
-#eval r6.rmatch "bb".toList
-#eval r6.gmatch "bb".toList
+#eval r6.matchEnd "bb"
+#eval r6.gmatch "bb"
 
--- (ε|b)(ε|b)*
+-- (ε + b)(ε + b)*
 def r6' : Regex (Char) := (epsilon.plus 'b').mul ((epsilon.plus 'b').star false)
-#eval r6'.rmatch "bb".toList
-#eval r6'.gmatch "bb".toList
+#eval r6'.matchEnd "bb"
+#eval r6'.gmatch "bb"
 
--- (a|ε|b)*
+-- (a + ε + b)*
 def r7 : Regex (Char) := (plus 'a' (epsilon.plus 'b')).star false
-#eval r7.rmatch "aaaabbb".toList
-#eval r7.gmatch "aaaabbb".toList
+#eval r7.matchEnd "aaaabbb"
+#eval r7.gmatch "aaaabbb"
 
--- (ε|a)b
+-- (ε + a)b
 def r8 : Regex (Char) := (epsilon.plus 'a').mul 'b'
-#eval r8.rmatch "ab".toList
-#eval r8.gmatch "ab".toList
+#eval r8.matchEnd "ab"
+#eval r8.gmatch "ab"
 
--- ((a|ε|b)|b)
+-- ((a + ε + b) + b)
 def r9 : Regex (Char) := Regex.plus ((plus 'a' epsilon).plus 'b') 'b'
-#eval r9.gmatch "b".toList
-#eval r9.rmatch "b".toList
+#eval r9.gmatch "b"
+#eval r9.matchEnd "b"
 
--- (ε|a)*b
+-- (ε + a)*b
 def r10 : Regex (Char) := ((Regex.plus epsilon 'a').star false).mul 'b'
-#eval r10.gmatch "ab".toList
-#eval r10.rmatch "ab".toList
+#eval r10.gmatch "ab"
+#eval r10.matchEnd "ab"
 
--- (a|ε)*(ε|b)
+-- (a + ε)*(ε + b)
 def r11 : Regex (Char) := ((Regex.plus 'a' epsilon).star false).mul (Regex.plus (epsilon) 'b')
-#eval r11.gmatch "ab".toList
-#eval r11.rmatch "ab".toList
+#eval r11.gmatch "ab"
+#eval r11.matchEnd "ab"
 
--- (ε|a)*(ε|b)
+-- (ε + a)*(ε + b)
 def r12 : Regex (Char) := ((Regex.plus epsilon 'a').star false).mul (Regex.plus (epsilon) 'b')
-#eval r12.gmatch "ab".toList
-#eval r12.rmatch "ab".toList
+#eval r12.gmatch "ab"
+#eval r12.matchEnd "ab"
 
--- (a|ε|b)*b
+-- (a + ε + b)*b
 def r13 : Regex (Char) := ((Regex.plus 'a' (Regex.plus epsilon 'b')).star false).mul 'b'
-#eval r13.gmatch "bb".toList
-#eval r13.rmatch "bb".toList
+#eval r13.gmatch "bb"
+#eval r13.matchEnd "bb"
 
 -- a*?a
 def r14 : Regex (Char) := (star 'a' true).mul 'a'
-#eval r14.rmatch "aaa".toList
-#eval r14.gmatch "aaa".toList
+#eval r14.matchEnd "aaa"
+#eval r14.gmatch "aaa"
 
 -- a*?b
 def r15 : Regex (Char) := (star 'a' true).mul 'b'
-#eval r15.rmatch "aab".toList
-#eval r15.gmatch "aab".toList
+#eval r15.matchEnd "aab"
+#eval r15.gmatch "aab"
 
--- (a|ε|b)*?b
+-- (a + ε + b)*?b
 def r16 : Regex (Char) := (star (plus 'a' (plus epsilon 'b')) true).mul 'b'
-#eval r16.rmatch "aabb".toList
-#eval r16.gmatch "aabb".toList
+#eval r16.matchEnd "aabb"
+#eval r16.gmatch "aabb"
 
+-- (aa + aaa)*
 def r17 : Regex (Char) := (star (plus "aa" "aaa") false)
-#eval r17.rmatch "aaa".toList
-#eval r17.gmatch "aaa".toList
+#eval r17.matchEnd "aaa"
+#eval r17.gmatch "aaa"
+
+-- (a + b*?)*
+def r18 : Regex Char := (star (plus 'a' (star 'b' true)) false)
+#eval r18.matchEnd "aaabbb"
+#eval r18.gmatch "aaabbb"
+
+-- (a* + b)*
+def r19 : Regex Char := (star (plus (star 'a' false) 'b') false)
+#eval r19.prune
+#eval r19.deriv 'a'
+#eval (r19.deriv 'a').prune
+#eval (r19.deriv 'a').prune.deriv 'b'
+
+-- (aa + aaa)*
+def r20 : Regex Char := (star (plus (mul 'a' 'a') (mul 'a' (mul 'a' 'a'))) false)
+#eval r20.prune
+#eval r20.deriv 'a'
+#eval (r20.deriv 'a').prune
+#eval (r20.deriv 'a').prune.deriv 'a'
