GreedyDeriv/Locations.lean
@@ -17,23 +17,3 @@ def Loc.word (loc : Loc α) : List α := loc.left.reverse ++ loc.right
 def Loc.reverse (loc : Loc α) : Loc α :=
   match loc with
   | ⟨u, v⟩ => ⟨v, u⟩
-
-abbrev Span (σ : Type u) := List σ × List σ × List σ
-
-@[simp]
-def Span.left (s : Span σ) : List σ := s.1
-
-@[simp]
-def Span.match (s : Span σ) : List σ := s.2.1
-
-@[simp]
-def Span.right (s : Span σ) : List σ := s.2.2
-
-@[simp]
-def Span.reverse (s : Span σ) : Span σ :=
-  match s with
-  | ⟨s, u, v⟩ => ⟨v, u.reverse, s⟩
-
-def merge_start_end (start_loc end_loc : Loc σ) : Span σ :=
-  match start_loc, end_loc with
-  | ⟨s, _⟩, ⟨u, v⟩ => ⟨s, u.reverse.drop s.length, v⟩
